src/panPredicateScript.sml
@@ -1,0 +1,95 @@
+(***********************************************************************
+ * Definitions and Proofs about Predicates on Pancake States           *
+ ***********************************************************************)
+
+Theory panPredicate
+Ancestors panSem
+
+fun elim_cases xs = EVERY (map (fn x => Cases_on x >> gvs[]) xs);
+
+Definition evaluates_def:
+  evaluates e s ⇔ ∃v. eval s e = SOME v
+End
+
+Definition evaluates_to_def:
+  evaluates_to e v s ⇔ eval s e = SOME v
+End
+
+Definition evaluates_to_word_def:
+  evaluates_to_word e s ⇔ ∃w. eval s e = SOME (ValWord w)
+End
+
+Definition evaluates_to_true_def:
+  evaluates_to_true e s ⇔ ∃w. eval s e = SOME (ValWord w) ∧ w ≠ 0w
+End
+
+Definition evaluates_to_false_def:
+  evaluates_to_false e s ⇔ ∃w. eval s e = SOME (ValWord w) ∧ w = 0w
+End
+
+Theorem evaluates_to_word_lem:
+  ∀e s. evaluates_to_word e s ⇒ evaluates_to_true e s ∨ evaluates_to_false e s
+Proof
+  rw[evaluates_to_word_def,evaluates_to_true_def,evaluates_to_false_def]
+  >> elim_cases [‘w = 0w’]
+QED
+
+Theorem evaluates_to_word_contradict:
+  ∀e s. evaluates_to_true  e s ⇒ ¬evaluates_to_false e s ∧
+        evaluates_to_false e s ⇒ ¬evaluates_to_true  e s
+Proof
+  rw[evaluates_to_true_def,evaluates_to_false_def]
+QED
+
+Definition valid_value_def:
+  valid_value k v e s ⇔ ∃value. eval s e = SOME value ∧
+                                case k of
+                                | Local  => is_valid_value s.locals  v value
+                                | Global => is_valid_value s.globals v value
+End
+
+Definition subst_def:
+  subst k v e P s ⇔ ∃value. eval s e = SOME value ∧
+                                   case k of
+                                   | Local  => P (s with locals  := s.locals  |+ (v,value))
+                                   | Global => P (s with globals := s.globals |+ (v,value))
+End
+
+Definition reset_local_subst_def:
+  reset_local_subst v s Q (r,t) ⇔ Q (r,t with locals := res_var t.locals (v,FLOOKUP s.locals v))
+End
+
+Definition knows_eid_def:
+  knows_eshape eid s ⇔ ∃sh. FLOOKUP s.eshapes eid = SOME sh
+End
+
+Definition has_eshape_def:
+  has_eshape eid sh s ⇔ FLOOKUP s.eshapes eid = SOME sh
+End
+
+Definition addr_in_mem_def:
+  addr_in_mem a v s ⇔ ∃m. mem_stores a (flatten v) s.memaddrs s.memory = SOME m
+End
+
+Definition mem_subst_def:
+  mem_subst a v P s ⇔ ∃m. mem_stores a (flatten v) s.memaddrs s.memory = SOME m ∧
+                          P (s with memory := m)
+End
+
+Definition addr_in_mem_32_def:
+  addr_in_mem_32 a v s ⇔ ∃m. mem_store_32 s.memory s.memaddrs s.be a (w2w v) = SOME m
+End
+
+Definition mem_subst_32_def:
+  mem_subst_32 a v P s ⇔ ∃m. mem_store_32 s.memory s.memaddrs s.be a (w2w v) = SOME m ∧
+                             P (s with memory := m)
+End
+
+Definition addr_in_mem_byte_def:
+  addr_in_mem_byte a v s ⇔ ∃m. mem_store_byte s.memory s.memaddrs s.be a (w2w v) = SOME m
+End
+
+Definition mem_subst_byte_def:
+  mem_subst_byte a v P s ⇔ ∃m. mem_store_byte s.memory s.memaddrs s.be a (w2w v) = SOME m ∧
+                               P (s with memory := m)
+End
